More_Mapping.thy
@@ -41,9 +41,18 @@ lemma lookupBool_update' [simp]:
 definition mapping_value_sum where
  "mapping_value_sum m = sum_list (map snd (Mapping.ordered_entries m))"
 
-lemma mapping_value_sum_update [simp]:
+lemma mapping_value_sum_update_plus [simp]:
   assumes "finite (Mapping.keys m)"
   shows "mapping_value_sum (Mapping.update k (lookupNat m k + v) m) = mapping_value_sum m + v"
+  using assms
+  sorry
+
+lemma mapping_value_sum_update_minus [simp]:
+  assumes "finite (Mapping.keys m)"
+  assumes "v \<le> lookupNat m k"
+  shows
+     "v \<le> mapping_value_sum m"
+     "mapping_value_sum (Mapping.update k (lookupNat m k - v) m) = mapping_value_sum m - v"
   using assms
   sorry
 
